seiostar/RQ.Metaprogram.Tests.ExamplesRefs.fst
@@ -9,7 +9,9 @@ open QTypes.HelperTactics
 
 open ExamplesRefs
 
-%splice_t[tgt_incr_int64] (generate_derivation "tgt_incr_int64" (`incr_int64))
+%splice_t[tgt_incr_nat8] (generate_derivation "tgt_incr_nat8" (`incr_nat8))
+
+%splice_t[tgt_incr_nat8'] (generate_derivation "tgt_incr_nat8'" (`incr_nat8'))
 
 %splice_t[tgt_refbool] (generate_derivation "tgt_refbool" (`refbool))
 %splice_t[tgt_falsepre] (generate_derivation "tgt_falsepre" (`falsepre))
